Combine some modules

Source/DafnyCore/Prelude/Boxes.dfy
@@ -1,8 +1,75 @@
 module Boxes {
   export
     provides Box, arbitrary
+    provides Below, Reflexive, Antisymmetric, Transitive, Total
+    provides Less, LessIrreflexive, LessAsymmetric, LessBelowAsymmetric, LessTransitive, Connected
 
   type Box(==,0,!new)
 
   const arbitrary: Box
+
+  /// The following predicate and 4 lemmas postulate a total order "Below" on Box'es.
+
+  predicate {:axiom} Below(a: Box, b: Box)
+
+  lemma {:axiom} Reflexive(a: Box)
+    ensures Below(a, a)
+
+  lemma {:axiom} Antisymmetric(a: Box, b: Box)
+    requires Below(a, b) && Below(b, a)
+    ensures a == b
+
+  lemma {:axiom} Transitive(a: Box, b: Box, c: Box)
+    requires Below(a, b) && Below(b, c)
+    ensures Below(a, c)
+
+  lemma {:axiom} Total(a: Box, b: Box)
+    ensures Below(a, b) || Below(b, a)
+
+  // strict order
+
+  predicate Less(a: Box, b: Box) {
+    Below(a, b) && a != b
+  }
+
+  lemma LessIrreflexive(a: Box)
+    ensures !Less(a, a)
+  {
+  }
+
+  lemma LessAsymmetric(a: Box, b: Box)
+    requires Less(a, b) && Less(b, a)
+    ensures false
+  {
+    Antisymmetric(a, b);
+  }
+
+  lemma LessBelowAsymmetric(a: Box, b: Box)
+    requires Less(a, b) && Below(b, a)
+    ensures false
+  {
+    Antisymmetric(a, b);
+  }
+
+  lemma LessTransitive(a: Box, b: Box, c: Box)
+    requires Less(a, b) && Less(b, c)
+    ensures Less(a, c)
+  {
+    assert Below(a, c) by {
+      Transitive(a, b, c);
+    }
+    assert a != c by {
+      if a == c {
+        Antisymmetric(a, b);
+        assert a == b;
+        assert false;
+      }
+    }
+  }
+
+  lemma Connected(a: Box, b: Box)
+    ensures a != b ==> Less(a, b) || Less(b, a)
+  {
+    Total(a, b);
+  }
 }
